Handle TProof correcly in L3/L4.
Add an App_e Prf_e a -> Prf_e reduction rule accordingly.
Changed L2k to translate TInd to a TProof, as these types
can be applied and we don't want to get reduction stuck because
of that. For TSort and TProd both TAx and TProof could be fine
but that would mean leaving axioms in later phases, for inert type
arguments, which does not seem necessary.

theories/L4_deBruijn/expression.v
@@ -63,7 +63,7 @@ Inductive exp: Type :=
 | Let_e: name -> exp -> exp -> exp
 | Fix_e: efnlst -> N -> exp  (* implicitly lambdas *)
 | Ax_e: string -> exp
-(* | Prf_e : exp *)
+| Prf_e : exp
 with exps: Type :=
 | enil: exps
 | econs: exp -> exps -> exps
@@ -132,6 +132,7 @@ Inductive exp_wf: N -> exp -> Prop :=
 | fix_e_wf: forall i (es:efnlst) k, efnlst_wf (efnlst_length es + i) es ->
                                      exp_wf i (Fix_e es k)
 (* Fix?: Axiom applied to anything should reduce to Axiom *)
+| prf_e_wf : forall i, exp_wf i Prf_e
 | ax_e_wf : forall i s, exp_wf i (Ax_e s)
 with exps_wf: N -> exps -> Prop :=
 | enil_wf: forall i, exps_wf i enil
@@ -219,6 +220,7 @@ Fixpoint shift n k e :=
     | Match_e e p bs => Match_e (shift n k e) p (shift_branches' shift n k bs)
     | Fix_e es k' => Fix_e (shift_efnlst shift n (efnlst_length es + k) es) k'
     | Ax_e s => Ax_e s
+    | Prf_e => Prf_e
   end.
 
 Definition shifts := shift_exps' shift.
@@ -280,6 +282,7 @@ Function subst (v:exp) k (e:exp): exp :=
     | Match_e e p bs => Match_e (subst v k e) p (subst_branches v k bs)
     | Fix_e es k' => Fix_e (subst_efnlst v (efnlst_length es + k) es) k'
     | Ax_e s => Ax_e s
+    | Prf_e => Prf_e
   end
 with substs (v:exp) k (es:exps) : exps :=
        match es with
@@ -311,6 +314,7 @@ Function sbst (v:exp) k (e:exp): exp :=
     | Match_e e p bs => Match_e (sbst v k e) p (sbst_branches v k bs)
     | Fix_e es k' => Fix_e (sbst_efnlst v (efnlst_length es + k) es) k'
     | Ax_e s => Ax_e s
+    | Prf_e => Prf_e
   end
 with sbsts (v:exp) k (es:exps) : exps :=
        match es with
@@ -547,6 +551,10 @@ Inductive eval: exp -> exp -> Prop :=
     enthopt (N.to_nat n) es = Some e' ->
     eval (App_e (sbst_fix es e') v2) e'' ->
     eval (App_e e e2) e''
+| eval_ProofApp_e : forall f a,
+    eval f Prf_e ->
+    eval (App_e f a) Prf_e
+| eval_Prf_e : eval Prf_e Prf_e
 (** Fix? :  (Ax _) --> Ax *)
 | eval_Ax_e s : eval (Ax_e s) (Ax_e s)
 with evals: exps -> exps -> Prop :=
@@ -578,6 +586,7 @@ Proof.
       assert (j1:v2 = v0). { apply H0. assumption. } subst.
       apply H1. assumption.
     * specialize (H _ H5); discriminate.
+    * specialize (H _ H6); discriminate.
   - inversion H0. subst. apply f_equal2. reflexivity.
     apply H. assumption.
   - inversion H1. subst.
@@ -594,6 +603,12 @@ Proof.
       specialize (H0 _ H6); subst v0.
       assert (e' = e'0) by congruence; subst e'0.
       now apply H1.
+    * specialize (H _ H6); discriminate.
+  - inversion H0; subst.
+    * specialize (H _ H3); discriminate.
+    * specialize (H _ H3); discriminate.
+    * reflexivity.
+  - inversion H. reflexivity.
   - inversion H. reflexivity.
   - inversion H. reflexivity.
   - inversion H1. subst. rewrite (H v0); try assumption.
@@ -638,6 +653,7 @@ Function eval_n (n:nat) (e:exp) {struct n}: option exp :=
     | S n => match e with
                | Lam_e na d => Some (Lam_e na d)
                | Fix_e es k => Some (Fix_e es k)
+               | Prf_e => Some Prf_e
                | Con_e d es => 
                  match evals_n n es with
                      | None => None
@@ -661,6 +677,7 @@ Function eval_n (n:nat) (e:exp) {struct n}: option exp :=
                        | _ => None
                        end
                      end
+                   | Some Prf_e => Some Prf_e
                    | _ => None
                   end
                | Let_e _ e1 e2 =>
@@ -853,6 +870,7 @@ Proof.
   intros; try discriminate.
   + injection H; intros h0. subst. constructor.
   + injection H; intros h0. subst. constructor.
+  + injection H. intros <-; constructor.
   + injection H0; intros h0. rewrite <- h0. constructor. apply H. assumption.
   + econstructor.
     * specialize (H _ e4). eapply H.
@@ -863,6 +881,8 @@ Proof.
     * specialize (H0 _ e5). apply H0.
     * apply e6.
     * now apply H1.
+  + subst.
+    injection H0. intros <-. specialize (H _ e4). econstructor 8; auto.
   + econstructor.
     * specialize (H _ e4). eapply H.
     * specialize (H0 _ H1). apply H0.
@@ -940,6 +960,8 @@ Proof.
     rewrite k0.
     replace (x0 + (x + x1 - 1))%nat with (x1 + (x + x0 - 1))%nat; try lia.
     rewrite e3, k1. reflexivity.
+  - destruct H as [x h]. exists (S x).
+    simpl. now rewrite h.
   - destruct H as [x h]. destruct H0 as [x0 h0].
     assert (j:=eval_n_Some_Succ _ _ _ h).
     assert (j0:=evals_n_Some_Succ _ _ _ h0).
@@ -1328,6 +1350,7 @@ Inductive is_value: exp -> Prop :=
 | lam_is_value: forall na e, is_value (Lam_e na e)
 | con_is_value: forall d es, are_values es -> is_value (Con_e d es)
 | fix_is_value: forall es k, is_value (Fix_e es k)
+| prf_is_value : is_value Prf_e
 | ax_is_value : forall s, is_value (Ax_e s)
 with are_values: exps -> Prop :=
 | enil_are_values: are_values enil
@@ -1361,6 +1384,7 @@ Fixpoint is_valueb (e:exp): bool :=
     | Let_e _ _ _ => false
     | Fix_e _ _ => true
     | Ax_e _ => true
+    | Prf_e => true
   end
 with are_valuesb (es:exps): bool :=
        match es with
@@ -1645,6 +1669,7 @@ Function maxFree (e:exp): Z :=
     | Match_e e p bs => Z.max (maxFree e) (maxFreeB bs)
     | Fix_e es k' => maxFreeF es - (Z.of_N (efnlst_length es))
     | Ax_e s => -1
+    | Prf_e => -1
   end
 with maxFreeC (es:exps) : Z :=
     match es with
